Prefix(:=<https://w3id.org/pmd/cto.owl#>)
Prefix(dce:=<http://purl.org/dc/elements/1.1/>)
Prefix(owl:=<http://www.w3.org/2002/07/owl#>)
Prefix(rdf:=<http://www.w3.org/1999/02/22-rdf-syntax-ns#>)
Prefix(xml:=<http://www.w3.org/XML/1998/namespace>)
Prefix(xsd:=<http://www.w3.org/2001/XMLSchema#>)
Prefix(rdfs:=<http://www.w3.org/2000/01/rdf-schema#>)
Prefix(dcterms:=<http://purl.org/dc/terms/>)


Ontology(<https://w3id.org/pmd/cto.owl>
Import(<https://w3id.org/pmd/cto/imports/log_import.owl>)
Import(<https://w3id.org/pmd/cto/imports/mwo_import.owl>)
Import(<https://w3id.org/pmd/cto/imports/pmdco_import.owl>)
Import(<https://w3id.org/pmd/cto/imports/tto_import.owl>)
Annotation(dcterms:creator "Soheil Molaei")
Annotation(dcterms:creator "https://orcid.org/0000-0002-3092-0532")
Annotation(dcterms:description "Creep Testing Ontology (CTO) has been developed for representing the creep testing process, testing equipment and setup requirements, test specimen characteristics, loading and environmental conditions (e.g. stress, temperature, atmosphere), time-dependent deformation behavior, and related testing parameters and measurement procedures according to DIN EN ISO 204 standard.")
Annotation(dcterms:license <https://creativecommons.org/licenses/unspecified>)
Annotation(dcterms:title "Creep Testing Ontology")
Annotation(rdfs:comment "Reused ontologies: BFO, RO, OBI, IAO, PMDco, NFDIcore, MWO, LOG, TTO")

Declaration(Class(<https://w3id.org/pmd/CTO_0000001>))
Declaration(Class(<https://w3id.org/pmd/CTO_2e6f3727_0ef5_4c0c_9aa0_7745ace4a590>))
Declaration(Class(<https://w3id.org/pmd/CTO_304180f6_5aa2_40d3_8430_21926d842d43>))
Declaration(Class(<https://w3id.org/pmd/CTO_314d2145_d087_4e58_b125_cd1afe4417d6>))
Declaration(Class(<https://w3id.org/pmd/CTO_33fc0e20_9b53_421f_8317_9fd1570290f2>))
Declaration(Class(<https://w3id.org/pmd/CTO_6c7ab730_4768_4e02_947d_d5640cf729b3>))
Declaration(Class(<https://w3id.org/pmd/CTO_71e6c975_af2c_4911_ae3c_f2c31ca92da8>))
Declaration(Class(<https://w3id.org/pmd/CTO_97b1b0e0_f4ed_4b50_a4ff_3a53ad181310>))
Declaration(Class(<https://w3id.org/pmd/CTO_a2a699e1_4865_4bb1_a259_76d9533f90f8>))
Declaration(Class(<https://w3id.org/pmd/CTO_c794f084_0123_467e_83ea_317faad81ad0>))
Declaration(Class(<https://w3id.org/pmd/CTO_d9f3408a_df31_4af5_a1de_33931741f97e>))
Declaration(Class(<https://w3id.org/pmd/CTO_e1e83721_4881_46c1_bf25_d7d1fb6fd94b>))
Declaration(AnnotationProperty(dcterms:description))
Declaration(AnnotationProperty(dcterms:license))
Declaration(AnnotationProperty(dcterms:title))
############################
#   Annotation Properties
############################

# Annotation Property: dcterms:description (description)

AnnotationAssertion(rdfs:label dcterms:description "description")

# Annotation Property: dcterms:license (license)

AnnotationAssertion(rdfs:label dcterms:license "license")

# Annotation Property: dcterms:title (title)

AnnotationAssertion(rdfs:label dcterms:title "title")



############################
#   Classes
############################

# Class: <https://w3id.org/pmd/CTO_0000001> (testing recipe)

AnnotationAssertion(rdfs:label <https://w3id.org/pmd/CTO_0000001> "testing recipe"@en)
AnnotationAssertion(<http://www.w3.org/2004/02/skos/core#definition> <https://w3id.org/pmd/CTO_0000001> "")
SubClassOf(<https://w3id.org/pmd/CTO_0000001> <https://w3id.org/pmd/co/PMD_0060008>)

# Class: <https://w3id.org/pmd/CTO_2e6f3727_0ef5_4c0c_9aa0_7745ace4a590> (planned test force)

AnnotationAssertion(rdfs:label <https://w3id.org/pmd/CTO_2e6f3727_0ef5_4c0c_9aa0_7745ace4a590> "planned test force"@en)
AnnotationAssertion(<http://www.w3.org/2004/02/skos/core#definition> <https://w3id.org/pmd/CTO_2e6f3727_0ef5_4c0c_9aa0_7745ace4a590> "The specific magnitude of force (Load) to be applied to the specimen.")
SubClassOf(<https://w3id.org/pmd/CTO_2e6f3727_0ef5_4c0c_9aa0_7745ace4a590> <https://w3id.org/pmd/CTO_0000001>)

# Class: <https://w3id.org/pmd/CTO_304180f6_5aa2_40d3_8430_21926d842d43> (planned preload)

AnnotationAssertion(rdfs:label <https://w3id.org/pmd/CTO_304180f6_5aa2_40d3_8430_21926d842d43> "planned preload"@en)
AnnotationAssertion(<http://www.w3.org/2004/02/skos/core#definition> <https://w3id.org/pmd/CTO_304180f6_5aa2_40d3_8430_21926d842d43> "A small initial load applied to align the specimen and remove \"slack\" from the fixture before the actual test starts.")
SubClassOf(<https://w3id.org/pmd/CTO_304180f6_5aa2_40d3_8430_21926d842d43> <https://w3id.org/pmd/CTO_0000001>)

# Class: <https://w3id.org/pmd/CTO_314d2145_d087_4e58_b125_cd1afe4417d6> (planned temperature)

AnnotationAssertion(rdfs:label <https://w3id.org/pmd/CTO_314d2145_d087_4e58_b125_cd1afe4417d6> "planned temperature"@en)
AnnotationAssertion(<http://www.w3.org/2004/02/skos/core#definition> <https://w3id.org/pmd/CTO_314d2145_d087_4e58_b125_cd1afe4417d6> "The target temperature at which the specimen is maintained throughout the test (critical in creep testing as creep is temperature-dependent).")
SubClassOf(<https://w3id.org/pmd/CTO_314d2145_d087_4e58_b125_cd1afe4417d6> <https://w3id.org/pmd/CTO_0000001>)

# Class: <https://w3id.org/pmd/CTO_33fc0e20_9b53_421f_8317_9fd1570290f2> (planned loading control type)

AnnotationAssertion(rdfs:label <https://w3id.org/pmd/CTO_33fc0e20_9b53_421f_8317_9fd1570290f2> "planned loading control type"@en)
AnnotationAssertion(<http://www.w3.org/2004/02/skos/core#definition> <https://w3id.org/pmd/CTO_33fc0e20_9b53_421f_8317_9fd1570290f2> "The feedback mechanism used to control the machine, typically Force Control (for creep) or Strain Control (for fatigue/relaxation).")
SubClassOf(<https://w3id.org/pmd/CTO_33fc0e20_9b53_421f_8317_9fd1570290f2> <https://w3id.org/pmd/CTO_0000001>)

# Class: <https://w3id.org/pmd/CTO_6c7ab730_4768_4e02_947d_d5640cf729b3> (planned interruption course)

AnnotationAssertion(rdfs:label <https://w3id.org/pmd/CTO_6c7ab730_4768_4e02_947d_d5640cf729b3> "planned interruption course"@en)
AnnotationAssertion(<http://www.w3.org/2004/02/skos/core#definition> <https://w3id.org/pmd/CTO_6c7ab730_4768_4e02_947d_d5640cf729b3> "A schedule for pausing the test to take manual measurements or inspect the specimen (e.g., cooling down and reheating).")
SubClassOf(<https://w3id.org/pmd/CTO_6c7ab730_4768_4e02_947d_d5640cf729b3> <https://w3id.org/pmd/CTO_0000001>)

# Class: <https://w3id.org/pmd/CTO_71e6c975_af2c_4911_ae3c_f2c31ca92da8> (planned test type)

AnnotationAssertion(rdfs:label <https://w3id.org/pmd/CTO_71e6c975_af2c_4911_ae3c_f2c31ca92da8> "planned test type"@en)
AnnotationAssertion(<http://www.w3.org/2004/02/skos/core#definition> <https://w3id.org/pmd/CTO_71e6c975_af2c_4911_ae3c_f2c31ca92da8> "The specific category of test, such as \"Tensile Creep,\" \"Compressive Creep,\" or \"Creep Rupture.\"")
SubClassOf(<https://w3id.org/pmd/CTO_71e6c975_af2c_4911_ae3c_f2c31ca92da8> <https://w3id.org/pmd/CTO_0000001>)

# Class: <https://w3id.org/pmd/CTO_97b1b0e0_f4ed_4b50_a4ff_3a53ad181310> (planned extension limit)

AnnotationAssertion(rdfs:label <https://w3id.org/pmd/CTO_97b1b0e0_f4ed_4b50_a4ff_3a53ad181310> "planned extension limit"@en)
AnnotationAssertion(<http://www.w3.org/2004/02/skos/core#definition> <https://w3id.org/pmd/CTO_97b1b0e0_f4ed_4b50_a4ff_3a53ad181310> "The maximum elongation (strain) allowed before the machine automatically stops the test to prevent damage or if the target is reached.")
SubClassOf(<https://w3id.org/pmd/CTO_97b1b0e0_f4ed_4b50_a4ff_3a53ad181310> <https://w3id.org/pmd/CTO_0000001>)

# Class: <https://w3id.org/pmd/CTO_a2a699e1_4865_4bb1_a259_76d9533f90f8> (planned loading type)

AnnotationAssertion(rdfs:label <https://w3id.org/pmd/CTO_a2a699e1_4865_4bb1_a259_76d9533f90f8> "planned loading type"@en)
AnnotationAssertion(<http://www.w3.org/2004/02/skos/core#definition> <https://w3id.org/pmd/CTO_a2a699e1_4865_4bb1_a259_76d9533f90f8> "The method of applying force, such as \"Constant Load\" (force remains the same) or \"Constant Stress\" (load is adjusted as the specimen cross-section changes).")
SubClassOf(<https://w3id.org/pmd/CTO_a2a699e1_4865_4bb1_a259_76d9533f90f8> <https://w3id.org/pmd/CTO_0000001>)

# Class: <https://w3id.org/pmd/CTO_c794f084_0123_467e_83ea_317faad81ad0> (planned initial stress)

AnnotationAssertion(rdfs:label <https://w3id.org/pmd/CTO_c794f084_0123_467e_83ea_317faad81ad0> "planned initial stress"@en)
AnnotationAssertion(<http://www.w3.org/2004/02/skos/core#definition> <https://w3id.org/pmd/CTO_c794f084_0123_467e_83ea_317faad81ad0> "The calculated stress applied to the specimen at the very start of the test.")
SubClassOf(<https://w3id.org/pmd/CTO_c794f084_0123_467e_83ea_317faad81ad0> <https://w3id.org/pmd/CTO_0000001>)

# Class: <https://w3id.org/pmd/CTO_d9f3408a_df31_4af5_a1de_33931741f97e> (planned test ending criterion)

AnnotationAssertion(rdfs:label <https://w3id.org/pmd/CTO_d9f3408a_df31_4af5_a1de_33931741f97e> "planned test ending criterion"@en)
AnnotationAssertion(<http://www.w3.org/2004/02/skos/core#definition> <https://w3id.org/pmd/CTO_d9f3408a_df31_4af5_a1de_33931741f97e> "The condition that triggers the end of the test, such as specimen rupture, reaching a specific strain (e.g., 1%), or a set duration.")
SubClassOf(<https://w3id.org/pmd/CTO_d9f3408a_df31_4af5_a1de_33931741f97e> <https://w3id.org/pmd/CTO_0000001>)

# Class: <https://w3id.org/pmd/CTO_e1e83721_4881_46c1_bf25_d7d1fb6fd94b> (planned time limit)

AnnotationAssertion(rdfs:label <https://w3id.org/pmd/CTO_e1e83721_4881_46c1_bf25_d7d1fb6fd94b> "planned time limit"@en)
AnnotationAssertion(<http://www.w3.org/2004/02/skos/core#definition> <https://w3id.org/pmd/CTO_e1e83721_4881_46c1_bf25_d7d1fb6fd94b> "The maximum duration the test is allowed to run if failure does not occur first.")
SubClassOf(<https://w3id.org/pmd/CTO_e1e83721_4881_46c1_bf25_d7d1fb6fd94b> <https://w3id.org/pmd/CTO_0000001>)


)